

Poisson Distribution

$$a) \quad p(X/k) = \frac{e^{-\lambda} \lambda^x}{x!}$$

$$p(y|\eta) = b(y) \exp(\eta^T T(y) - a(\eta))$$

$$p(x/k) = \frac{e^{\eta \ln k} \cdot e^{-\lambda}}{x!}$$

$$= \frac{1}{x!} \exp(x \ln k - \lambda)$$

$$b(\eta) = \frac{1}{x!}, \quad T(x) = x, \quad \eta^T = \ln k, \quad a(\eta) = \lambda$$

$$\eta = \ln k \rightarrow k = e^\eta$$

$$a(\eta) = \lambda = e^\eta$$

Canonical
Response
Function

$$g(\eta) = a'(\eta) = e^\eta$$

$$E(T(y)) = g(\eta) = e^\eta = \lambda$$

$$b) \quad y = d(1, 2, \dots, k) \in \mathbb{Z}$$

$$T(y)_1 = \begin{bmatrix} 1 \\ 0 \\ 0 \\ \vdots \end{bmatrix} \quad T(y)_2 = \begin{bmatrix} 0 \\ 1 \\ 0 \\ \vdots \end{bmatrix} \dots T(y)_{k-1} = \begin{bmatrix} 0 \\ 0 \\ \vdots \\ 1 \end{bmatrix}$$

$$p(y=1; \phi) = \phi_1, \quad p(y=2; \phi) = \phi_2 \dots p(y=k; \phi) = \phi_{k-1}$$

$$p(y=k; \phi) = 1 - \sum_{i=1}^{k-1} \phi_i$$

$$p(y; \phi) = \phi_1^{T(y)_1} \cdot \phi_2^{T(y)_2} \cdot \phi_3^{T(y)_3} \dots \phi_k^{1 - \sum_{i=1}^{k-1} T(y)_i}$$

$$= \exp \left(T(y)_1 \ln \phi_1 + T(y)_2 \ln \phi_2 \dots \left(1 - \sum_{i=1}^{k-1} T(y)_i \right) \ln \phi_k \right)$$

$$= \exp \left(T(y)_1 \ln \left(\frac{\phi_1}{\phi_k} \right) + T(y)_2 \ln \left(\frac{\phi_2}{\phi_k} \right) \dots + \ln \phi_k \right)$$

$$= b(y) \exp (\eta^T T(y) - a(\eta))$$

$$b(y)=1, \quad \eta^T = \left[\ln \left(\frac{\phi_1}{\phi_k} \right) \quad \ln \left(\frac{\phi_2}{\phi_k} \right) \quad \dots \quad \ln \left(\frac{\phi_{k-1}}{\phi_k} \right) \right]$$

$$a(\eta) = -\ln(\phi_k)$$

$$\eta_i = \ln \left(\frac{\phi_i}{\phi_R} \right) \rightarrow \phi_i = \phi_R e^{\eta_i}$$

$$\phi_R \sum_1^R e^{\eta_i} = \sum_1^R \phi_i = 1$$

$$\phi_R = \frac{1}{\sum_1^R e^{\eta_i}}$$

$$\text{So, } \phi_i = \frac{e^{\eta_i}}{\sum_{j=1}^R e^{\eta_j}}$$

$$p(y=i/q) = \phi_i = \frac{e^{\eta_i}}{\sum_{j=1}^R e^{\eta_j}}$$

$$p(y/q) = \prod_{i=1}^R \phi_i^{T(y)_i}$$

$$\ell(\theta) = \sum_{i=1}^R T(y)_i \phi_i$$